Improve unfolding tactic for the cases where a top-level identifier is applied to some implicit parameters.
It may happen that the user calls the unfolding command on an identifier
"id" which is actually an identifier applied to some implicit
parameters, in which case we need to strip the implicit parameters in
order to retrieve the top-level identifier.

FEM.Process.fst
@@ -2503,6 +2503,13 @@ let rec replace_term_in dbg from_term to_term tm =
     (* Unknown *)
     tm
 
+val strip_implicit_parameters : term -> Tac term
+let rec strip_implicit_parameters tm =
+  match inspect tm with
+  | Tv_App hd (a,qualif) ->
+    if Q_Implicit? qualif then strip_implicit_parameters hd else tm
+  | _ -> tm
+
 val unfold_in_assert_or_assume : bool -> exploration_result term -> Tac unit
 let unfold_in_assert_or_assume dbg ares =
   print_dbg dbg ("[> unfold_in_assert_or_assume:\n" ^ term_to_string ares.res);
@@ -2560,7 +2567,7 @@ let unfold_in_assert_or_assume dbg ares =
                  "- focused term: " ^ term_to_string unf_res.res);
   (* Unfold the term *)
   let res_view = inspect unf_res.res in
-  let ge1, unf_tm =
+  let ge1, opt_unf_tm =
     match res_view with
     | Tv_FVar fv ->
       print_dbg dbg ("The focused term is a top identifier: " ^ fv_to_string fv);
@@ -2568,7 +2575,7 @@ let unfold_in_assert_or_assume dbg ares =
       let fname = flatten_name (inspect_fv fv) in
       let subterm' = norm_term_env ares.ge.env [delta_only [fname]] subterm in
       print_dbg dbg ("Normalized subterm: " ^ term_to_string subterm');
-      ares.ge, subterm'
+      ares.ge, Some subterm'
     | _ ->
       (* Look for an equality given by a previous post-condition. In the case
        * the term is a bv, we can also use the let-binding which introduces it,
@@ -2588,21 +2595,46 @@ let unfold_in_assert_or_assume dbg ares =
       in
       let ge1, eq_tm = find_context_equality dbg ares.ge unf_res.res parents [] in
       (* Check if we found an equality *)
-      let eq_tm =
+      let opt_eq_tm =
         match eq_tm with
-        | Some eq_tm -> eq_tm
-        | _ ->
-          mfail ("unfold_in_assert_or_assume: " ^
-                 "couldn't find equalities with which to rewrite: " ^
-                 term_to_string unf_res.res)
+        | Some eq_tm -> Some eq_tm
+        | _ -> None
       in
       (* Apply it *)
       let subterm' =
-        match opt_bv with
-        | Some bv -> apply_subst ge1.env subterm [(bv, eq_tm)]
-        | None -> replace_term_in dbg unf_res.res eq_tm subterm
+        match opt_bv, opt_eq_tm with
+        | Some bv, Some eq_tm -> Some (apply_subst ge1.env subterm [(bv, eq_tm)])
+        | None, Some eq_tm -> Some (replace_term_in dbg unf_res.res eq_tm subterm)
+        | _ -> None
       in
       ge1, subterm'
+  in
+  (* If we couldn't unfold the term, check if it is a top-level identifier with
+   * implicit parameters (it may happen that the user calls the command on a
+   * top-level identifier which has implicit parameters without providing
+   * those parameters, in which case the focused term is the identifier applied
+   * to those implicits inferred by F*, and thus an app and not an fvar).
+   * Note that so far we have no way to check if the implicit parameters have
+   * been explicitly provided by the user or not, which is why we can't do better
+   * than greedy tests.*)
+  let ge2, unf_tm =
+    match opt_unf_tm with
+    | Some unf_tm -> ge1, unf_tm
+    | None ->
+      begin match inspect (strip_implicit_parameters unf_res.res) with
+      | Tv_FVar fv ->
+        print_dbg dbg ("The focused term is a top identifier with implicit parameters: "
+                       ^ fv_to_string fv);
+        (* The easy case: just use the normalizer *)
+        let fname = flatten_name (inspect_fv fv) in
+        let subterm' = norm_term_env ge1.env [delta_only [fname]] subterm in
+        print_dbg dbg ("Normalized subterm: " ^ term_to_string subterm');
+        ge1, subterm'
+      | _ ->        
+        mfail ("unfold_in_assert_or_assume: " ^
+               "couldn't find equalities with which to rewrite: " ^
+               term_to_string unf_res.res)
+      end
   in
   (* Create the assertions to output *)
   let final_assert = rebuild unf_tm in
@@ -2611,9 +2643,9 @@ let unfold_in_assert_or_assume dbg ares =
     if insert_before then mk_assertions [final_assert] [] else mk_assertions [] [final_assert]
   in
   (* Introduce fresh variables for the shadowed ones and substitute *)
-  let ge2, asserts = subst_shadowed_with_abs_in_assertions dbg ge1 None asserts in
+  let ge3, asserts = subst_shadowed_with_abs_in_assertions dbg ge2 None asserts in
   (* Output *)
-  printout_success ge2 asserts
+  printout_success ge3 asserts
 
 [@plugin]
 val pp_unfold_in_assert_or_assume : bool -> unit -> Tac unit
